added SHL

src/Dafny/bitwiseBinaryOperations.i.dfy
@@ -8,21 +8,53 @@ module bitwise_binary_operations_i {
     import opened types
     import opened conversion_operations_i
 
-    // TODO: REWRITE WITH BINOPS
-     function evalLSHR(op1:Data,op2:Data): (out:Data) // still wip
+    function evalLSHR(op1:Data,op2:Data): (out:Data) // still wip
         requires isInt(op1) && isInt(op2)
         requires op1.itype.size*8 > op2.val //See note above
         requires op2.val > 0
         ensures out.Int?;
         ensures out.itype.size == op1.itype.size && !out.itype.signed;
-     {
-        reveal_IntFits();
-        reveal_rightShift();
-        var initial := if op1.itype.signed then ToTwosComp(op1).val else op1.val;
-        var result := rightShift(initial,op2.val);
-        ValToData(result,op1.itype.size,false)
+    {
+        reveal_BitsToWord();
+        reveal_WordToBits();
+        if op1.itype.size == 1 then evalLSHR8(op1,op2) else 
+        if op1.itype.size == 2 then evalLSHR16(op1,op2) else 
+        if op1.itype.size == 4 then evalLSHR32(op1,op2) else 
+        evalLSHR64(op1,op2) 
+    }
 
-     }
+    function evalSHL(op1:Data,op2:Data): (out:Data) // still wip
+        requires isInt(op1) && isInt(op2)
+        requires op1.itype.size*8 > op2.val //See note above
+        requires op2.val > 0
+        ensures out.Int?;
+        ensures out.itype.size == op1.itype.size 
+        ensures out.itype.signed == op1.itype.signed
+    {
+        reveal_BitsToWord();
+        reveal_WordToBits();
+        if op1.itype.size == 1 then evalSHL8(op1,op2) else 
+        if op1.itype.size == 2 then evalSHL16(op1,op2) else 
+        if op1.itype.size == 4 then evalSHL32(op1,op2) else 
+        evalSHL64(op1,op2) 
+    }
+
+
+    // TODO: REWRITE WITH BINOPS
+    //  function evalLSHR(op1:Data,op2:Data): (out:Data) // still wip
+    //     requires isInt(op1) && isInt(op2)
+    //     requires op1.itype.size*8 > op2.val //See note above
+    //     requires op2.val > 0
+    //     ensures out.Int?;
+    //     ensures out.itype.size == op1.itype.size && !out.itype.signed;
+    //  {
+    //     reveal_IntFits();
+    //     reveal_rightShift();
+    //     var initial := if op1.itype.signed then ToTwosComp(op1).val else op1.val;
+    //     var result := rightShift(initial,op2.val);
+    //     ValToData(result,op1.itype.size,false)
+
+    //  }
     function {:opaque} rightShift(val:int,shift:int) : (result:int)
         requires shift >= 1
         requires val >= 0
@@ -69,6 +101,134 @@ module bitwise_binary_operations_i {
 
     }
 /// HELPER FUNCTIONS
+    // LSHR HELPER FUNCTIONS //
+function evalLSHR8(op1:Data,op2:Data): (out:Data)
+        requires isInt(op1) && isInt(op2)
+        requires op1.itype.size*8 > op2.val //See note above
+        requires op2.val > 0
+        requires op1.itype.size == 1
+        ensures out.Int?;
+        ensures out.itype.size == op1.itype.size && !out.itype.signed;
+     {
+        reveal_ToTwosComp(); 
+        reveal_IntFits();
+        reveal_BitShiftRight8();
+        var result := RightShiftByte(ToTwosComp(op1).val,ToTwosComp(op2).val);
+        ValToData(result,1,false)      
+     } 
+function evalLSHR16(op1:Data,op2:Data): (out:Data)
+        requires isInt(op1) && isInt(op2)
+        requires op1.itype.size*8 > op2.val //See note above
+        requires op2.val > 0
+        requires op1.itype.size == 2
+        ensures out.Int?;
+        ensures out.itype.size == op1.itype.size && !out.itype.signed;
+     {
+        reveal_ToTwosComp(); 
+        reveal_IntFits();
+        reveal_BitShiftRight16();
+        var result := RightShiftHalfWord(ToTwosComp(op1).val,ToTwosComp(op2).val);
+        ValToData(result,2,false)      
+     } 
+function evalLSHR32(op1:Data,op2:Data): (out:Data)
+        requires isInt(op1) && isInt(op2)
+        requires op1.itype.size*8 > op2.val //See note above
+        requires op2.val > 0
+        requires op1.itype.size == 4
+        ensures out.Int?;
+        ensures out.itype.size == op1.itype.size && !out.itype.signed;
+     {
+        reveal_ToTwosComp(); 
+        reveal_IntFits();
+        reveal_BitShiftRight();
+        var result := RightShift(ToTwosComp(op1).val,ToTwosComp(op2).val);
+        ValToData(result,4,false)      
+     }
+function evalLSHR64(op1:Data,op2:Data): (out:Data)
+        requires isInt(op1) && isInt(op2)
+        requires op1.itype.size*8 > op2.val //See note above
+        requires op2.val > 0
+        requires op1.itype.size == 8
+        ensures out.Int?;
+        ensures out.itype.size == op1.itype.size && !out.itype.signed;
+     {
+        reveal_ToTwosComp(); 
+        reveal_IntFits();
+        reveal_BitShr64();
+        var result := BitwiseShr64(ToTwosComp(op1).val,ToTwosComp(op2).val);
+        ValToData(result,8,false)      
+     }       
+       
+// SHL HELPER FUNCTIONS //
+function evalSHL8(op1:Data,op2:Data): (out:Data)
+        requires isInt(op1) && isInt(op2)
+        requires op1.itype.size*8 > op2.val //See note above
+        requires op2.val > 0
+        requires op1.itype.size == 1
+        ensures out.Int?;
+        ensures out.itype.size == op1.itype.size
+         ensures out.itype.signed == op1.itype.signed
+     {
+        reveal_ToTwosComp(); 
+        reveal_IntFits();
+        reveal_BitShiftLeft8();
+        var result := LeftShiftByte(ToTwosComp(op1).val,ToTwosComp(op2).val);
+        var unsigned := ValToData(result,1,false);
+        if  op1.itype.signed then FromTwosComp(unsigned) else unsigned
+      
+     } 
+function evalSHL16(op1:Data,op2:Data): (out:Data)
+        requires isInt(op1) && isInt(op2)
+        requires op1.itype.size*8 > op2.val //See note above
+        requires op2.val > 0
+        requires op1.itype.size == 2
+        ensures out.Int?;
+        ensures out.itype.size == op1.itype.size 
+         ensures out.itype.signed == op1.itype.signed
+     {
+        reveal_ToTwosComp(); 
+        reveal_IntFits();
+        reveal_BitShiftLeft16();
+        var result := LeftShiftHalfWord(ToTwosComp(op1).val,ToTwosComp(op2).val);
+        var unsigned := ValToData(result,2,false);  
+        if  op1.itype.signed then FromTwosComp(unsigned) else unsigned
+    
+     } 
+function evalSHL32(op1:Data,op2:Data): (out:Data)
+        requires isInt(op1) && isInt(op2)
+        requires op1.itype.size*8 > op2.val //See note above
+        requires op2.val > 0
+        requires op1.itype.size == 4
+        ensures out.Int?;
+        ensures out.itype.size == op1.itype.size
+        ensures out.itype.signed == op1.itype.signed
+     {
+        reveal_ToTwosComp(); 
+        reveal_IntFits();
+        reveal_BitShiftLeft();
+        var result := LeftShift(ToTwosComp(op1).val,ToTwosComp(op2).val);
+        var unsigned := ValToData(result,4,false);
+        if  op1.itype.signed then FromTwosComp(unsigned) else unsigned
+      
+     }
+function evalSHL64(op1:Data,op2:Data): (out:Data)
+        requires isInt(op1) && isInt(op2)
+        requires op1.itype.size*8 > op2.val //See note above
+        requires op2.val > 0
+        requires op1.itype.size == 8
+        ensures out.Int?;
+        ensures out.itype.size == op1.itype.size
+        ensures out.itype.signed == op1.itype.signed
+     {
+        reveal_ToTwosComp(); 
+        reveal_IntFits();
+        reveal_BitShl64();
+        var result := BitwiseShl64(ToTwosComp(op1).val,ToTwosComp(op2).val);
+        // if op1.itype.signed then ValToData(result,8,false)   
+        var unsigned := ValToData(result,8,false);
+        if  op1.itype.signed then FromTwosComp(unsigned) else unsigned
+     }       
+       
     // AND HELPER FUNCTIONS //
 function evalAND8(dstSize:bitWidth,op1:Data,op2:Data): (out:Data)
       requires isInt(op1) && isInt(op2)
@@ -185,27 +345,66 @@ function evalOR64(dstSize:bitWidth,op1:Data,op2:Data): (out:Data)
      // --  Lemmas for correctness checking -----
     lemma evalSHLIsValid()
     {
-       
+        reveal_BitShl64();
+        reveal_BitShiftLeft();
+        reveal_BitShiftLeft16();
+        reveal_BitShiftLeft8();
+        reveal_BitsToWord();
+        reveal_WordToBits();
+        reveal_ByteToBits();
+        reveal_BitsToByte();
+        reveal_FromTwosComp();
+        // <<result> = shl i32 4, 2      ; yields i32: 16
+         var v0:uint32 := 4;
+         var v1:uint32 := 2;
+         var d0:uint32 := 2;
+         var out:Data := evalSHL(UInt32(v0),UInt32(v1));
+         assert out.itype.size == 4;// == UInt64(d0);
+         assert WordToBits(v0) == 4;
+         assert WordToBits(v1) == 2;
+         assert out.val == 16;
+
+         //<result> = shl i32 1, 10     ; yields i32: 1024
+         var v2:uint32 := 1;
+         var v3:uint32 := 10;
+         var d1:uint32 := 1;
+         var out1:Data := evalSHL(UInt32(v2),UInt32(v3));
+         assert out1.itype.size == 4;// == UInt64(d0);
+         assert ByteToBits(ToTwosComp(UInt8(v3)).val) == 10;
+         assert BitShiftLeft(WordToBits(v2),v3) == 1024;
+         assert out1.val == 1024;
+
+         //<result> = shl i32 1, 10     ; yields i32: 1024
+         var v4:sint8 := -4;
+         var v5:uint8 := 4;
+         var out2:Data := evalSHL(SInt8(v4),UInt8(v5));
+         assert out2.itype.size == 1;// == UInt64(d0);
+        //  assert ByteToBits(ToTwosComp(UInt8(v3)).val) == 10;
+        assert ByteToBits(ToTwosComp(SInt8(v4)).val) == 252;
+        assert BitShiftLeft8(ByteToBits(ToTwosComp(SInt8(v4)).val),v5) == 192;
+        assert out2.val == -64;
     }
 
     lemma evalLSHRIsValid()
     {
-        reveal_IntFits();
-        reveal_IntFromBytes();
-        reveal_IntToBytes();
-        reveal_ExtendZeroBytes();
-        reveal_rightShift();
-        reveal_WordToBits64();
-        reveal_BitsToWord64();
-        reveal_ToTwosComp();
+        reveal_BitShr64();
+        reveal_BitShiftRight();
+        reveal_BitShiftRight16();
+        reveal_BitShiftRight8();
+        reveal_BitsToWord();
+        reveal_WordToBits();
+        reveal_ByteToBits();
+        reveal_BitsToByte();
         // <result> = lshr i32 4, 1   ; yields i32:result = 2
          var v0:uint32 := 4;
          var v1:uint32 := 1;
          var d0:uint32 := 2;
          var out:Data := evalLSHR(UInt32(v0),UInt32(v1));
          assert out.itype.size == 4;// == UInt64(d0);
+         assert WordToBits(v0) == 4;
+         assert WordToBits(v1) == 1;
          assert out.val == 2;
-         assert out.val == UInt32(d0).val;
+        //  assert out.val == UInt32(d0).val;
 
         // <result> = lshr i32 4, 2   ; yields i32:result = 1
          var v2:uint32 := 4;
@@ -214,7 +413,7 @@ function evalOR64(dstSize:bitWidth,op1:Data,op2:Data): (out:Data)
          var out1:Data := evalLSHR(UInt32(v2),UInt32(v3));
          assert out1.itype.size == 4;// == UInt64(d0);
          assert out1.val == 1;
-         assert out1.val == UInt32(d1).val;
+        //  assert out1.val == UInt32(d1).val;
 
         // <result> = lshr i8  4, 3   ; yields i8:result = 0
          var v4:uint32 := 4;
@@ -223,25 +422,29 @@ function evalOR64(dstSize:bitWidth,op1:Data,op2:Data): (out:Data)
          var out2:Data := evalLSHR(UInt32(v4),UInt32(v5));
          assert out2.itype.size == 4;// == UInt64(d0);
          assert out2.val == 0;
-         assert out2.val == UInt32(d2).val;
+        //  assert out2.val == UInt32(d2).val;
          
         // <result> = lshr i8 -2, 1   ; yields i8:result = 0x7F
          var v6:sint8 := -2;
-         var v7:uint32 := 1;
+         var v7:sint8 := 1;
          var d3:uint8 := 127;
          var out3:Data := evalLSHR(SInt8(v6),UInt32(v7));
          assert out3.itype.size == 1;// == UInt64(d0);
          assert out3.val == 127;
-         assert out3.val == UInt8(d3).val;
+        //  assert out3.val == UInt8(d3).val;
 
          // <result> = lshr i8 -2, 1   ; yields i8:result = 0x7F
          var v8:sint8 := -42;
-         var v9:uint32 := 2;
+         var v9:sint8 := 2;
          var d4:uint8 := 53;
-         var out4:Data := evalLSHR(SInt8(v8),UInt32(v9));
+         var out4:Data := evalLSHR(SInt8(v8),SInt32(v9));
          assert out4.itype.size == 1;// == UInt64(d0);
+         assert ByteToBits(ToTwosComp(SInt8(v8)).val) == 214;
+        //  assert ByteToBits(ToTwosComp(UInt8(v9)).val) == 2;
+        // assert ToTwosComp(SInt8(v8)).val == 214;
+
          assert out4.val == 53;
-         assert out4.val == UInt8(d4).val;
+        //  assert out4.val == UInt8(d4).val;
 
         //
        
